theories/sim/local.v
@@ -11,7 +11,7 @@ Variable (wsat: A → state → state → Prop).
 Variable (vrel: A → expr → expr → Prop).
 Variable (fns fnt: fn_env).
 
-Definition rrel (vrel: A → expr → expr → Prop)(r: A) (es et: expr) : Prop :=
+Definition rrel (vrel: A → expr → expr → Prop) (r: A) (es et: expr) : Prop :=
   ∀ vt, to_result et = Some vt → ∃ vs, to_result es = Some vs ∧
     match vs, vt with
     | ValR vs, ValR vt => vrel r (Val vs) (Val vt)
@@ -20,83 +20,82 @@ Definition rrel (vrel: A → expr → expr → Prop)(r: A) (es et: expr) : Prop 
     | _, _ => False
     end.
 
-Inductive _sim_local_body_step (r_f : A)
-  (sim_local_body : A → nat → expr → state → expr → state → Prop)
-  (r: A) (idx: nat) : expr → state → expr → state → Prop :=
+Notation PRED := (A → nat → expr → state → expr → state → Prop)%type.
+Notation SIM := (A → nat → expr → state → expr → state → PRED → Prop)%type.
+
+Implicit Type (Φ: PRED).
+
+Inductive _sim_local_body_step (r_f : A) (sim_local_body : SIM)
+  (r: A) (idx: nat) es σs et σt Φ : Prop :=
 (* If tgt makes 1 step, src can make some step *)
-| sim_local_body_step_next e_src σ_src e_tgt σ_tgt
-    (STEP: ∀ e_tgt' σ_tgt'
-      (STEPT: (e_tgt, σ_tgt) ~{fnt}~> (e_tgt', σ_tgt')),
+| sim_local_body_step_next
+    (STEP: ∀ et' σt' (STEPT: (et, σt) ~{fnt}~> (et', σt')),
       (* then we locally can makes some step and pick a new resource r' *)
-      ∃ e_src' σ_src' r' idx',
-        ((e_src, σ_src) ~{fns}~>+ (e_src', σ_src') ∨
-         ((idx' < idx)%nat ∧ (e_src', σ_src') = (e_src, σ_src))) ∧
-        wsat (r_f ⋅ r') σ_src' σ_tgt' ∧
-        sim_local_body r' idx' e_src' σ_src' e_tgt' σ_tgt')
-    : _sim_local_body_step r_f sim_local_body r idx e_src σ_src e_tgt σ_tgt
+      ∃ es' σs' r' idx',
+        ((es, σs) ~{fns}~>+ (es', σs') ∨
+         ((idx' < idx)%nat ∧ (es', σs') = (es, σs))) ∧
+        wsat (r_f ⋅ r') σs' σt' ∧
+        sim_local_body r' idx' es' σs' et' σt' Φ)
 (* If tgt prepares to make a call to [name], src should be able to make the same
   call. Here we do not want to step into the call of [name], but to step over it. *)
 | sim_local_body_step_over_call
-    (K_src: list (ectxi_language.ectx_item (bor_ectxi_lang fns)))
-    (K_tgt: list (ectxi_language.ectx_item (bor_ectxi_lang fnt)))
-    fid e_src e_tgt el_tgt σ_src σ_tgt
-    (CALLTGT: e_tgt = fill K_tgt (Call #[ScFnPtr fid] el_tgt))
+    (Ks: list (ectxi_language.ectx_item (bor_ectxi_lang fns)))
+    (Kt: list (ectxi_language.ectx_item (bor_ectxi_lang fnt)))
+    fid el_tgt
+    (CALLTGT: et = fill Kt (Call #[ScFnPtr fid] el_tgt))
     (STEPOVER: ∀
       (* tgt is ready to make a call of [name] *)
       (VTGT : Forall (λ ei, is_Some (to_value ei)) el_tgt),
       (* then src is also ready to make a call of [name] *)
       ∃ el_src σ1_src rc rv,
-      (e_src, σ_src) ~{fns}~>*
-        (fill K_src (Call #[ScFnPtr fid] el_src), σ1_src) ∧
+      (es, σs) ~{fns}~>*
+        (fill Ks (Call #[ScFnPtr fid] el_src), σ1_src) ∧
       Forall (λ ei, is_Some (to_value ei)) el_src ∧
       (* and we can pick a resource [rv] for the arguments *)
-      wsat (r_f ⋅ (rc ⋅ rv)) σ1_src σ_tgt ∧
+      wsat (r_f ⋅ (rc ⋅ rv)) σ1_src σt ∧
       (* [rv] justifies the arguments *)
       Forall2 (vrel rv) el_src el_tgt ∧
       (* and after the call our context can continue *)
-      (∀ r' v_src v_tgt σ_src' σ_tgt'
+      (∀ r' v_src v_tgt σs' σt'
         (* For any new resource r' that supports the returned values are
           related w.r.t. (r ⋅ r' ⋅ r_f) *)
         (VRET: vrel r' (Val v_src) (Val v_tgt)),
         ∃ idx', sim_local_body (rc ⋅ r') idx'
-                                (fill K_src (Val v_src)) σ_src'
-                                (fill K_tgt (Val v_tgt)) σ_tgt'))
-    : _sim_local_body_step r_f sim_local_body r idx e_src σ_src e_tgt σ_tgt.
+                                (fill Ks (Val v_src)) σs'
+                                (fill Kt (Val v_tgt)) σt' Φ)).
 
-Record sim_local_body_base
-  (r_f: A) (sim_local_body : A → nat → expr → state → expr → state → Prop)
-  (r: A) (idx: nat) e_src σ_src e_tgt σ_tgt : Prop := {
+Record sim_local_body_base (r_f: A) (sim_local_body : SIM)
+  (r: A) (idx: nat) es σs et σt Φ : Prop := {
   sim_local_body_terminal :
     (* if tgt is terminal *)
-    terminal e_tgt →
+    terminal et →
       (* then src can get terminal *)
-      ∃ e_src' σ_src' r', (e_src, σ_src) ~{fns}~>* (e_src', σ_src') ∧
-        terminal e_src' ∧
+      ∃ es' σs' r', (es, σs) ~{fns}~>* (es', σs') ∧
+        terminal es' ∧
         (* and re-establish wsat *)
-        wsat (r_f ⋅ r') σ_src' σ_tgt ∧ Wf σ_src' ∧
+        wsat (r_f ⋅ r') σs' σt ∧ Wf σs' ∧
         (* and the returned values are related *)
-        rrel vrel r' e_src' e_tgt ;
+        rrel vrel r' es' et ∧ ∃ idx', Φ r' idx' es' σs' et σt ;
   sim_local_body_step :
-      _sim_local_body_step r_f sim_local_body r idx e_src σ_src e_tgt σ_tgt
+      _sim_local_body_step r_f sim_local_body r idx es σs et σt Φ
 }.
 
-Inductive _sim_local_body
-  (sim_local_body : A → nat → expr → state → expr → state → Prop)
-  (r: A) (idx: nat) (e_src: expr) (σ_src: state) (e_tgt: expr) (σ_tgt: state) : Prop :=
+Inductive _sim_local_body (sim_local_body : SIM)
+  (r: A) (idx: nat) es σs et σt Φ : Prop :=
 (* If src is stuck, then anything is related *)
 | sim_local_body_stuck
-    (STUCK: stuck (Λ:=bor_lang fns) e_src σ_src)
+    (STUCK: stuck (Λ:=bor_lang fns) es σs)
 (* Otherwise, either tgt is terminal or makes 1 step, src can make some steps *)
 | sim_local_body_not_stuck
     (STEP: ∀ r_f
       (* for any frame r_f that is compatible with our resource r 
         has world satisfaction *)
-      (WSAT: wsat (r_f ⋅ r) σ_src σ_tgt),
-      sim_local_body_base r_f sim_local_body r idx e_src σ_src e_tgt σ_tgt).
+      (WSAT: wsat (r_f ⋅ r) σs σt),
+      sim_local_body_base r_f sim_local_body r idx es σs et σt Φ).
 
-Lemma sim_local_body_mono : monotone6 _sim_local_body.
+Lemma sim_local_body_mono : monotone7 _sim_local_body.
 Proof.
-  intros r idx es σs et σt R R' SIM LE; inversion SIM; subst.
+  intros r idx es σs et σt Φ R R' SIM LE; inversion SIM; subst.
   { by eapply sim_local_body_stuck; eauto. }
   eapply sim_local_body_not_stuck. intros.
   destruct (STEP _ WSAT) as [TM ST]. split; [naive_solver|].
@@ -105,35 +104,30 @@ Proof.
   - econstructor 2; eauto. naive_solver.
 Qed.
 
-Definition sim_local_body := paco6 _sim_local_body bot6.
+Definition sim_local_body := paco7 _sim_local_body bot7.
 
-(* Simulating functions: assuming the calls have been initialized. *)
+(* Simulating functions:
+  - We start after the substitution.
+  - We assume the arguments are values related by [r]
+  - The returned result must also be values and related by [vrel]. *)
 Definition sim_local_fun (fn_src fn_tgt : function) : Prop :=
-  ∀ r e_src e_tgt el_src el_tgt σ_src σ_tgt
+  ∀ r es et el_src el_tgt σs σt
     (VALS: Forall (λ ei, is_Some (to_value ei)) el_src)
     (VALT: Forall (λ ei, is_Some (to_value ei)) el_tgt)
     (VALEQ: Forall2 (vrel r) el_src el_tgt)
     (EQS: match fn_src with
-          | FunV xl e => subst_l xl el_src e = Some e_src
+          | FunV xl e => subst_l xl el_src e = Some es
           end)
     (EQT: match fn_tgt with
-          | FunV xl e => subst_l xl el_tgt e = Some e_tgt
+          | FunV xl e => subst_l xl el_tgt e = Some et
           end),
-    ∃ idx, sim_local_body r idx (InitCall e_src) σ_src (InitCall e_tgt) σ_tgt.
+    ∃ idx, sim_local_body r idx (InitCall es) σs (InitCall et) σt
+                          (λ r _ es _ et _, vrel r es et).
 
 Definition sim_local_funs : Prop :=
   ∀ name fn_src, fns !! name = Some fn_src → ∃ fn_tgt,
     fnt !! name = Some fn_tgt ∧ sim_local_fun fn_src fn_tgt.
 
-Definition init_state := (mkState ∅ ∅ [] O O).
-(* Program simulation: All functions are related, and so is initialization. *)
-Record sim_prog := {
-  sim_prog_env: sim_local_funs;
-  sim_prog_main:
-    ∃ idx, sim_local_body ε idx
-                          (Call #["main"] []) init_state
-                          (Call #["main"] []) init_state;
-}.
 End local.
 
 Hint Resolve sim_local_body_mono : paco.
