theories/sim/one_step.v
@@ -5,22 +5,26 @@ From stbor.sim Require Import local invariant.
 
 Set Default Proof Using "Type".
 
-Lemma local_update_discrete_valid_frame `{CmraDiscrete A} (r_f r r' : A) :
-  ✓ (r_f ⋅ r) → (r_f ⋅ r, r) ~l~> (r_f ⋅ r', r') → ✓ (r_f ⋅ r').
-Proof.
-  intros VALID UPD. apply cmra_discrete_valid.
-  apply (UPD O (Some r_f)); [by apply cmra_discrete_valid_iff|by rewrite /= comm].
-Qed.
+Notation "r ⊨{ n , fs , ft } ( es , σs ) ≤ ( et , σt ) : Φ" :=
+  (sim_local_body wsat vrel_expr fs ft r n%nat es%E σs et%E σt Φ)
+  (at level 70, format "r  ⊨{ n , fs , ft }  ( es ,  σs )  ≤  ( et ,  σt )  :  Φ").
 
-Notation sim_body := (sim_local_body wsat vrel_expr).
-Notation sim_fun := (sim_local_fun wsat vrel_expr).
-Notation sim_funs := (sim_local_funs wsat vrel_expr).
+Notation "⊨{ fs , ft } f1 ≤ᶠ f2" :=
+  (sim_local_fun wsat vrel_expr fs ft f1 f2)
+  (at level 70, format "⊨{ fs , ft }  f1  ≤ᶠ  f2").
 
 Instance dom_proper `{Countable K} {A : cmraT} :
   Proper ((≡) ==> (≡)) (dom (M:=gmap K A) (gset K)).
 Proof.
   intros m1 m2 Eq. apply elem_of_equiv. intros i.
   by rewrite !elem_of_dom Eq.
+Qed.
+
+Lemma local_update_discrete_valid_frame `{CmraDiscrete A} (r_f r r' : A) :
+  ✓ (r_f ⋅ r) → (r_f ⋅ r, r) ~l~> (r_f ⋅ r', r') → ✓ (r_f ⋅ r').
+Proof.
+  intros VALID UPD. apply cmra_discrete_valid.
+  apply (UPD O (Some r_f)); [by apply cmra_discrete_valid_iff|by rewrite /= comm].
 Qed.
 
 (* Lemma sim_body_head_step fns fnt r n
@@ -31,20 +35,19 @@ Qed.
   sim_body fns fnt r n (fill Ks es) σs (fill Kt et) σt.
 Proof. *)
 
-Lemma sim_body_init_call fns fnt r n es et σs σt :
+Lemma sim_body_init_call fs ft r n es et σs σt Φ :
   let σs' := mkState σs.(shp) σs.(sst) (σs.(snc) :: σs.(scs)) σs.(snp) (S σs.(snc)) in
   let σt' := mkState σt.(shp) σt.(sst) (σt.(snc) :: σt.(scs)) σt.(snp) (S σt.(snc)) in
   let r'  : resUR := (∅, {[σt.(snc) := to_callStateR (csOwned ∅)]}) in
-  sim_body fns fnt (r ⋅ r') n (EndCall es) σs' (EndCall et) σt' →
-  sim_body fns fnt r n (InitCall es) σs (InitCall et) σt.
+  r ⋅ r' ⊨{n,fs,ft} (EndCall es, σs') ≤ (EndCall et, σt') : Φ →
+  r ⊨{n,fs,ft} (InitCall es, σs) ≤ (InitCall et, σt) : Φ.
 Proof.
-  intros σs' σt' r' SIM. pfold.
+  intros σs' σt1 r' SIM. pfold.
   constructor 2. intros. split; [by intros []|]. constructor 1.
   intros.
   exists (EndCall es), σs', (r ⋅ r').
-  destruct (tstep_init_call_inv _ _ _ _ _ STEPT).
-  subst e_tgt' σ_tgt'.
-  have STEPS: (InitCall es, σs) ~{fns}~> (EndCall es, σs').
+  destruct (tstep_init_call_inv _ _ _ _ _ STEPT). subst et' σt'.
+  have STEPS: (InitCall es, σs) ~{fs}~> (EndCall es, σs').
   { by eapply (head_step_tstep _ []), initcall_head_step. }
   have FRESH: (r_f ⋅ r).2 !! σt.(snc) = None.
   { destruct ((r_f ⋅ r).2 !! σt.(snc)) as [cs|] eqn:Eqcs; [|done].
@@ -106,7 +109,7 @@ Proof.
   intros ST. split; [by apply fill_not_val, ST|apply irreducible_fill; apply ST].
 Qed.
 
-Lemma sim_body_end_call fns fnt r n es et σs σt :
+(* Lemma sim_body_end_call fns fnt r n es et σs σt :
   sim_body fns fnt r n es σs et σt →
   sim_body fns fnt r n (EndCall es) σs (EndCall et) σt.
 Proof.
@@ -123,4 +126,4 @@ Proof.
     destruct (TE Tet) as
       (es' & σs1 & r1 & STEPS1 & Tes1 & WSAT1).
     exists es, (mkState σs1.(shp) σs1.(sst) cids σs1.(snp) σs1.(snc)).
-Abort.
+Abort. *)
